VLSM/Equivocators/MessageProperties.v
@@ -54,7 +54,6 @@ Proof.
   destruct (le_lt_dec (S n) j); try discriminate Hitem.
   destruct descriptorx as [s | i' [|]] eqn:Hl; simpl.
   - destruct (nat_eq_dec (S j) (S n)); try discriminate Hitem.
-    inversion Hitem. subst. clear Hitem. repeat split; reflexivity.
   - destruct (nat_eq_dec (S j) (S n)); try discriminate Hitem.
     inversion Hitem. subst. repeat split; reflexivity.
   - destruct (nat_eq_dec i' j); try discriminate Hitem.
@@ -104,14 +103,22 @@ Lemma preloaded_equivocator_vlsm_trace_project_protocol_item
   (bitem : vtransition_item equivocator_vlsm)
   (Hitem : In bitem btr)
   (fi : bool)
-  : exists
-    (d d' : MachineDescriptor)
-    (item : vtransition_item X)
-    (Hitem : equivocator_vlsm_transition_item_project _ bitem d = Some (Some item, d'))
-    (tr : list (vtransition_item X))
-    (dfinal dfirst : MachineDescriptor)
-    (Htr : equivocator_vlsm_trace_project _ btr dfinal = Some (tr, dfirst)),
-    In item tr.
+  : match snd (l bitem) with
+    | NewMachine _ sn =>
+      exists
+      (d : MachineDescriptor)
+      (Hitem : equivocator_vlsm_transition_item_project _ bitem d = Some (None, snd (l bitem))),
+      input bitem = None /\ output bitem = None
+    | _ =>
+      exists
+      (d : MachineDescriptor)
+      (item : vtransition_item X)
+      (Hitem : equivocator_vlsm_transition_item_project _ bitem d = Some (Some item, snd (l bitem)))
+      (tr : list (vtransition_item X))
+      (dfinal dfirst : MachineDescriptor)
+      (Htr : equivocator_vlsm_trace_project _ btr dfinal = Some (tr, dfirst)),
+      In item tr
+    end.
 Proof.
   apply in_split in Hitem.
   destruct Hitem as [bprefix [bsuffix Heq]].
@@ -140,59 +147,57 @@ Proof.
     (equivocator_protocol_transition_item_project_inv5 _ l s lst iom oom Hv Ht) as Hpitem.
   replace (@Build_transition_item message (@type message (@Common.equivocator_vlsm message X)) l iom s oom)
     with bitem in Hpitem.
+  unfold Common.l in *.
+  destruct l as [l dl].
+  unfold snd in *.
   rewrite H in *.
-  destruct (Hpitem false) as [i [Hi [d' [itemx _Hitemx]]]].
-  pose (dfinal := Existing X i false).
-  destruct
-    (preloaded_equivocator_vlsm_trace_project_protocol_inv _ _ _ H2 _ Hi false)
-    as [fsuffix [suffix Hsuffix]].
-  specialize (Hpitem fsuffix).
-  destruct Hpitem as [_i [_Hi [_d' [_itemx Hitemx]]]].
+  destruct dl as [sndl | idl fdl].
+  - spec Hpitem false. destruct Hpitem as [i [Hi Hpitem]].
+    eexists _. exists Hpitem.
+    simpl in Ht. unfold vtransition in Ht. simpl in Ht.
+    inversion Ht. destruct Hv as [Hsndl Hiom].
+    subst. split; reflexivity.
+  - destruct (Hpitem false) as [i [Hi [itemx Hitemx]]].
+    pose (dfinal := Existing X i false).
+    destruct
+      (preloaded_equivocator_vlsm_trace_project_protocol_inv _ _ _ H2 _ Hi false)
+      as [fsuffix [suffix Hsuffix]].
+    specialize (Hpitem fsuffix).
+  destruct Hpitem as [_i [_Hi [_itemx _Hitemx]]].
   destruct
     (equivocator_vlsm_transition_item_project_some_inj _ Hitemx _Hitemx)
-    as [H_i [H_itemx H_d']].
-  subst _i _itemx _d'. clear _Hitemx. clear _Hi.
-  exists (Existing _ i fsuffix). exists d'. exists itemx. exists Hitemx.
+    as [H_i [H_itemx _]].
+  subst _i _itemx. clear Hitemx. clear _Hi.
+  exists (Existing _ i fsuffix). exists itemx. exists _Hitemx.
   remember (Existing _ i fsuffix) as dsuffix.
   assert (Hitem : equivocator_vlsm_trace_project _ [bitem] dsuffix = equivocator_vlsm_trace_project _ [bitem] dsuffix)
     by reflexivity.
   remember [bitem] as lbitem. rewrite Heqlbitem in Hitem at 2.
   simpl in Hitem.
-  rewrite Hitemx in Hitem.
+  rewrite _Hitemx in Hitem.
   specialize
     (equivocator_vlsm_trace_project_app_inv _ _ _ _ _ _ _ _ Hitem Hsuffix)
     as Hsuffix'.
-  rewrite <- H in Hitemx.
+  rewrite <- H in _Hitemx.
   destruct
-    (equivocator_protocol_transition_item_project_inv2 _ l lst s iom oom Hv Ht _ _ _ Hitemx)
+    (equivocator_protocol_transition_item_project_inv2 _ (l, Existing _ idl fdl) lst s iom oom Hv Ht _ _ _ _Hitemx)
     as [_i [_fi [_Hdsuffix [_Hi [Heqitemx Hd']]]]].
   rewrite Heqdsuffix in _Hdsuffix. inversion _Hdsuffix. subst _i _fi. clear _Hdsuffix.
   replace (of_nat_lt _Hi) with (of_nat_lt Hi) in *; try apply of_nat_ext. clear _Hi.
-  destruct d' as [sn | id fd].
-  - destruct Hd' as [Hsn [Hvsn Htsn]].
-    assert
-      (Hprefix : equivocator_vlsm_trace_project  _ bprefix (NewMachine _ sn) = Some ([], NewMachine _ sn))
-      by apply equivocator_vlsm_trace_project_on_new_machine.
-    specialize
-      (equivocator_vlsm_trace_project_app_inv _ _ _ _ _ _ _ _ Hprefix Hsuffix')
-      as Htr.
-    subst lbitem.
-    simpl in Htr.
-    exists (itemx :: suffix).
-    exists dfinal. exists (NewMachine _ sn). exists Htr. left. reflexivity.
-  - destruct Hd' as [Hid [Hvs' Hts']].
-    subst lst.
-    destruct
-      (preloaded_equivocator_vlsm_trace_project_protocol _ _ _ Hbprefix id Hid fd)
-      as [prefix [dfirst [Hprefix _]]].
-    specialize
-      (equivocator_vlsm_trace_project_app_inv _ _ _ _ _ _ _ _ Hprefix Hsuffix')
-      as Htr.
-    subst lbitem.
-    simpl in Htr.
-    exists (prefix ++ itemx :: suffix).
-    exists dfinal. exists dfirst. exists Htr.
-    apply in_app_iff. right. left. reflexivity.
+  destruct Hd' as [_i' [_fi' [_Heq [id [Hvs' Hts']]]]].
+  inversion _Heq. subst _i' _fi'. clear _Heq.
+  subst lst.
+  destruct
+    (preloaded_equivocator_vlsm_trace_project_protocol _ _ _ Hbprefix idl id fdl)
+    as [prefix [dfirst [Hprefix _]]].
+  specialize
+    (equivocator_vlsm_trace_project_app_inv _ _ _ _ _ _ _ _ Hprefix Hsuffix')
+    as Htr.
+  subst lbitem.
+  simpl in Htr.
+  exists (prefix ++ itemx :: suffix).
+  exists dfinal. exists dfirst. exists Htr.
+  apply in_app_iff. right. left. reflexivity.
 Qed.
 
 (**
@@ -214,15 +219,17 @@ Lemma equivocator_vlsm_trace_project_output_reflecting_inv
 Proof.
   apply Exists_exists in Hbbs.
   destruct Hbbs as [item [Hin Houtput]].
-  destruct
+  specialize
     (preloaded_equivocator_vlsm_trace_project_protocol_item _ _ Htr _ Hin false)
-    as [i [i' [itemx [Hitemx [trx [ifinal [ifirst [Htrx Hinx]]]]]]]].
+    as Hitem.
+  destruct (snd (l item)) as [sn | i fi] eqn:Hsndl
+  ; try (destruct Hitem as [_ [_ [_ Hcontra]]]; congruence).
+  destruct Hitem as [d [itemx [Hitemx [trx [ifinal [ifirst [Htrx Hinx]]]]]]].
   exists ifinal. exists ifirst. exists trx. exists Htrx.
   apply Exists_exists. exists itemx. split; try assumption.
   apply equivocator_transition_item_project_inv_messages in Hitemx.
   destruct Hitemx as [_ [_ [_ [_ Hitemx]]]].
-  simpl in *.
-  rewrite Hitemx in Houtput. assumption.
+  congruence.
 Qed.
 
 Section has_been_sent_lifting.
@@ -438,7 +445,7 @@ Definition equivocator_has_been_sent_capability
   {|
     has_been_sent := equivocator_has_been_sent;
     proper_sent := equivocator_proper_sent;
-    proper_not_sent := equivocator_proper_not_sent   
+    proper_not_sent := equivocator_proper_not_sent
   |}.
 
 End has_been_sent_lifting.
@@ -454,7 +461,7 @@ Context
   (Hbeen_sent_X := @computable_sent_messages_has_been_sent_capability message X Hsent_messages message_eq)
   .
 
-(** We define the [sent_messages_fn] for the [equivocator_vlsm] as the 
+(** We define the [sent_messages_fn] for the [equivocator_vlsm] as the
 union of all [sent_messages_fn] for its internal machines.
 *)
 Definition equivocator_sent_messages_fn
@@ -554,7 +561,7 @@ Qed.
 
 (** Finally, we define the [computable_sent_messages] instance for the
 [equivocator_vlsm].
-Note that we can reuse the consistency property proved above since 
+Note that we can reuse the consistency property proved above since
 [computable_sent_messages] for <<X>> implies [has_been_sent_capability].
 *)
 Definition equivocator_computable_sent_messages
